# Sample Exam

## 1.1

P0, P1, and P3 are the same.  
(Divide (x, y, z) by w).  
P2 is differing.

## P0

$$\begin{pmatrix}  3\\ 4\\ 2\\ 0.5 \end{pmatrix} = \begin{pmatrix} 3/0.5\\ 4/0.5\\ 2/0.5\\ 0.5/0.5 \end{pmatrix} = \begin{pmatrix}  6\\ 8\\ 4\\ 1 \end{pmatrix}$$

## P1

$$\begin{pmatrix}  24\\ 32\\ 16\\ 4 \end{pmatrix} = \begin{pmatrix} 24/4\\ 32/4\\ 16/4\\ 4/4 \end{pmatrix} = \begin{pmatrix}  6\\ 8\\ 4\\ 1 \end{pmatrix}$$

1.2:Â 

![[Pasted image 20230426153643.png]]

Normal: $$T(d) * R(90) * T(-c)$$
$$T = \begin{pmatrix}  0 &   \end{pmatrix} * \begin{pmatrix}   cos(\theta) & -sin(\theta) & 0\\   sin(\theta) & cos(\theta)  & 0\\ 0 & 0 & 1\end{pmatrix}$$
  
Inverse: $$T(-c) * R(90) * T(d)$$
